{
    "@context": {
        "trl": "https://w3id.org/research-technology-readiness-level#",
        "skos": "http://www.w3.org/2004/02/skos/core#",
        "rdf": "http://www.w3.org/1999/02/22-rdf-syntax-ns#",
        "rdfs": "http://www.w3.org/2000/01/rdf-schema#"
    },
    "@graph": [
        {
            "@id": "trl:Levels",
            "@type": "skos:OrderedCollection",
            "skos:memberList": [
                "tlr:Stage1Planning",
                "tlr:Stage2ProofOfConcept",
                "tlr:Stage3Experimental",
                "tlr:Stage4Complete",
                "tlr:Level0Idea",
                "tlr:Level1InitialResearch",
                "tlr:Level2ConceptFormulated",
                "tlr:Level3ProofOfConcept",
                "trl:Level4ValidatedProofOfConcept",
                "trl:Level5EarlyPrototype",
                "trl:Level6LatePrototype",
                "trl:Level7ReleaseCandidate",
                "trl:Level8Complete",
                "trl:Level9Proven"
            ]
        },
        {
            "@id": "trl:Stages",
            "@type": "skos:OrderedCollection",
            "skos:memberList": [
                "tlr:Stage1Planning",
                "tlr:Stage2ProofOfConcept",
                "tlr:Stage3Experimental",
                "tlr:Stage4Complete"
            ]
        },
        {
            "@id": "tlr:Scheme",
            "@type": "skos:ConceptScheme"
        },
        {
            "@id": "tlr:TechnologyReadinessLevel",
            "@type": "rdfs:Class"
        },
        {
            "@id": "trl:Stage1Planning",
            "@type": [ "skos:Concept", "tlr:TechnologyReadinessLevel" ],
            "skos:inScheme": "tlr:Scheme",
            "skos:prefLabel": "Planning",
            "skos:altLabel": "pre-alpha",
            "skos:notation": "0-2",
            "skos:definition": "The technology is in an initial planning stage (pre-alpha), no implementation is available yet"
        },
        {
            "@id": "trl:Stage2ProofOfConcept",
            "@type": [ "skos:Concept", "tlr:TechnologyReadinessLevel" ],
            "skos:inScheme": "tlr:Scheme",
            "skos:prefLabel": "Proof of Concept",
            "skos:altLabel": "alpha",
            "skos:notation": "3-4",
            "skos:definition": "An initial proof-of-concept implementation of the technology is available (alpha). It is not mature enough for end-users yet."
        },
        {
            "@id": "trl:Stage3Experimental",
            "@type": [ "skos:Concept", "tlr:TechnologyReadinessLevel" ],
            "skos:inScheme": "tlr:Scheme",
            "skos:prefLabel": "Experimental",
            "skos:altLabel": "beta",
            "skos:notation": "5-7",
            "skos:definition": "The technology is implemented and ready for experimental settings (beta), but requires further work and validation."
        },
        {
            "@id": "trl:Stage4Complete",
            "@type": [ "skos:Concept", "tlr:TechnologyReadinessLevel" ],
            "skos:inScheme": "tlr:Scheme",
            "skos:prefLabel": "Complete",
            "skos:altLabel": "stable",
            "skos:notation": "8-9",
            "skos:definition": "The technology is complete, stable and deployed in production scenarios for end-users"
        },
        {
            "@id": "trl:Level0Idea",
            "@type": [ "skos:Concept", "tlr:TechnologyReadinessLevel" ],
            "skos:inScheme": "tlr:Scheme",
            "skos:prefLabel": "0 - Idea",
            "skos:notation": "0",
            "skos:definition": "Unproven, untested and largely unformulated concept",
            "skos:broader": "trl:Stage1Planning"
        },
        {
            "@id": "trl:Level1InitialResearch",
            "@type": [ "skos:Concept", "tlr:TechnologyReadinessLevel" ],
            "skos:inScheme": "tlr:Scheme",
            "skos:prefLabel": "1 - Initial Research",
            "skos:notation": "1",
            "skos:definition": "Basic (scholarly) needs observed and reported",
            "skos:broader": "trl:Stage1Planning"
        },
        {
            "@id": "trl:Level2ConceptFormulated",
            "@type": [ "skos:Concept", "tlr:TechnologyReadinessLevel" ],
            "skos:inScheme": "tlr:Scheme",
            "skos:prefLabel": "2 - Concept Formulated",
            "skos:notation": "2",
            "skos:definition": "Initial technology/application has seen concept formulated",
            "skos:broader": "trl:Stage1Planning"
        },
        {
            "@id": "trl:Level3ProofOfConcept",
            "@type": [ "skos:Concept", "tlr:TechnologyReadinessLevel" ],
            "skos:inScheme": "tlr:Scheme",
            "skos:prefLabel": "3 - Proof of Concept",
            "skos:notation": "3",
            "skos:definition": "Initial Proof-of-concept of key functionality. Concept presented for initial feedback from scholarly users. Not yet validated and not suitable for end-users yet.",
            "skos:broader": "trl:Stage2ProofOfConcept"
        },
        {
            "@id": "trl:Level4ValidatedProofOfConcept",
            "@type": [ "skos:Concept", "tlr:TechnologyReadinessLevel" ],
            "skos:inScheme": "tlr:Scheme",
            "skos:prefLabel": "4 - Validated Proof of Concept",
            "skos:notation": "4",
            "skos:definition": "Validated Proof-of-concept of key functionality. Technology validated in its own experimental setting (e.g. the lab). Not mature enough for end-users yet.",
            "skos:broader": "trl:Stage2ProofOfConcept"
        },
        {
            "@id": "trl:Level5EarlyPrototype",
            "@type": [ "skos:Concept", "tlr:TechnologyReadinessLevel" ],
            "skos:inScheme": "tlr:Scheme",
            "skos:prefLabel": "5 - Early Prototype",
            "skos:notation": "5",
            "skos:definition": "Technology validated in target setting (e.g. with potential end-users)",
            "skos:broader": "trl:Stage3Experimental"
        },
        {
            "@id": "trl:Level6LatePrototype",
            "@type": [ "skos:Concept", "tlr:TechnologyReadinessLevel" ],
            "skos:inScheme": "tlr:Scheme",
            "skos:prefLabel": "6 - Late prototype",
            "skos:notation": "6",
            "skos:definition": "Technology demonstrated in target setting, end-users adopt it for testing purposes.",
            "skos:broader": "trl:Stage3Experimental"
        },
        {
            "@id": "trl:Level7ReleaseCandidate",
            "@type": [ "skos:Concept", "tlr:TechnologyReadinessLevel" ],
            "skos:inScheme": "tlr:Scheme",
            "skos:prefLabel": "7 - Release Candidate",
            "skos:notation": "7",
            "skos:definition": "Technology ready enough and in initial use by end-users in intended scholarly environments. Further validation may be in progress.",
            "skos:broader": "trl:Stage3Experimental"
        },
        {
            "@id": "trl:Level8Complete",
            "@type": [ "skos:Concept", "tlr:TechnologyReadinessLevel" ],
            "skos:inScheme": "tlr:Scheme",
            "skos:prefLabel": "8 - Complete",
            "skos:notation": "8",
            "skos:definition": "Technology complete and qualified, released for all end-users in scholarly environments.",
            "skos:broader": "trl:Stage4Complete"
        },
        {
            "@id": "trl:Level9Proven",
            "@type": [ "skos:Concept", "tlr:TechnologyReadinessLevel" ],
            "skos:inScheme": "tlr:Scheme",
            "skos:prefLabel": "9 - Proven",
            "skos:notation": "9",
            "skos:definition": "Technology complete and proven in practice by real users.",
            "skos:broader": "trl:Stage4Complete"
        },
        {
            "@id": "tlr:technologyReadinessLevel",
            "@type": "rdf:Property",
            "rdfs:label": "Technology Readiness Level",
            "rdfs:comment": "Associates a technology readiness level (or a stage grouping several levels) with a subject (e.g. schema:SoftwareSourceCode or schema:SoftwareApplication). Takes a value (skos:Concept) from collection tlr:Levels (in conceptscheme tlr:Scheme)",
            "rdfs:range": "tlr:TechnologyReadinessLevel" 
        }
    ]
}
